theories/LogicalRelation/Transitivity.v
@@ -1,0 +1,137 @@
+From LogRel.AutoSubst Require Import core unscoped Ast Extra.
+From LogRel Require Import Notations Utils BasicAst Context Untyped Weakening GenericTyping LogicalRelation Reduction.
+From LogRel.LogicalRelation Require Import Induction ShapeView Reflexivity Irrelevance.
+
+Set Universe Polymorphism.
+
+Section Transitivity.
+Context `{GenericTypingProperties}.
+
+Set Printing Primitive Projection Parameters.
+
+Set Printing Universes.
+
+Lemma transEq@{i j k l} {Γ A B C lA lB lC} 
+  {RA : [LogRel@{i j k l} lA | Γ ||- A]}
+  {RB : [LogRel@{i j k l} lB | Γ ||- B]}
+  {RC : [LogRel@{i j k l} lC | Γ ||- C]}
+  (RAB : [Γ ||-<lA> A ≅ B | RA])
+   (RBC : [Γ ||-<lB> B ≅ C | RB]) :
+  [Γ ||-<lA> A ≅ C | RA].
+Proof.
+  destruct RA as [pA lrA], RB as [pB lrB], RC as [pC lrC]; cbn in *.
+  set (sv := combine _ _ _ _ lrA lrB lrC (ShapeViewConv _ _ RAB) (ShapeViewConv _ _ RBC)).
+  revert lB B pB lrB lC C pC lrC RAB RBC sv.
+  induction lrA as [| |?? ΠA ΠAad ihdom ihcod]; intros ??? lrB;
+  induction lrB as [|?? neB|?? ΠB ΠBad _ _]; intros ??? lrC;
+  induction lrC as [| |?? ΠC ΠCad _ _]; intros RAB RBC [].
+  - easy.
+  - destruct RAB as [tB red], RBC as [tC]; exists tC. 1,2: assumption.
+    etransitivity. 1: eassumption. destruct neB as [? red']. cbn in *.
+    unshelve erewrite (redtywf_det _ _ _ _ _ _ red red').
+    1,2 : apply whnf_whne. all: assumption.
+  - destruct RAB as [nB domB codB redB ? domRedEq codRedEq], RBC as [nC domC codC redC ? domRedEq' codRedEq'].
+    destruct ΠB as [??? redB' ??? domRedB codRedB], ΠC as [??? redC' ??? domRedC codRedC], ΠBad as [domAdB codAdB], ΠCad as [domAdC codAdC]; cbn in *.
+    unshelve epose proof (eqΠB := redtywf_det _ _ _ _ _ _ redB' redB).  1,2 : constructor.
+    injection eqΠB; intros eqcod eqdom eqna; clear eqΠB;  subst. 
+    unshelve epose proof (eqΠC := redtywf_det _ _ _ _ _ _ redC' redC).  1,2 : constructor.
+    injection eqΠC; intros eqcod eqdom eqna; clear eqΠC;  subst. 
+    assert (domRedAC : forall (Δ : context) (ρ : Δ ≤ Γ) (h : [ |-[ ta ] Δ]),
+      [PiRedTy.domRed ΠA ρ h | Δ ||- (PiRedTy.dom ΠA)⟨ρ⟩ ≅ domC⟨ρ⟩]).
+    { intros. unshelve eapply ihdom.
+      10: now unshelve apply domRedEq'.
+      7: apply domRedEq.
+      6: now unshelve apply domAdC.
+      3: apply domAdB.
+      now apply (PiRedTy.domRed ΠA).
+    }
+    exists nC domC codC.
+    + eassumption.
+    + etransitivity; eassumption.
+    + apply domRedAC.
+    + intros. unshelve eapply ihcod.
+      10:{ 
+        unshelve apply codRedEq'. 1: assumption. 
+        eapply RedTmConv.
+        4: exact ha.
+        * apply (PiRedTy.domAd ΠAad).
+        * apply domAdB.
+        * apply domRedEq.
+      }
+      7: unshelve apply codRedEq.
+      6:{ unshelve apply codAdC. 1: assumption.
+        eapply RedTmConv.
+        4: exact ha.
+        * apply (PiRedTy.domAd ΠAad).
+        * apply domAdC.
+        * apply domRedAC.
+      }
+      3: apply codAdB.
+      now eapply (PiRedTy.codRed ΠA).
+Qed.
+
+
+Lemma transEqTermU@{h i j k} {Γ l t u v} {h : [Γ ||-U l]} :
+  [LogRelRec@{i j k} l | Γ ||-U t ≅ u :U| h] ->
+  [LogRelRec@{i j k} l | Γ ||-U u ≅ v :U| h] ->
+  [LogRelRec@{i j k} l | Γ ||-U t ≅ v :U| h].
+Proof.
+  intros [rL ?? redL] [? rR] ; exists rL rR redL; tea.
+  + etransitivity; tea.
+    unshelve erewrite (redtmwf_det _ _ _ _ _ _ _ _ (URedTm.red redR) (URedTm.red redL0))  ; tea.
+    all: apply isType_whnf; apply URedTm.type.
+  + apply TyEqRecFwd; unshelve eapply transEq@{h i j k}.
+    6,7: now apply (TyEqRecFwd h). 
+    2: apply (RedTyRecFwd h); tea.
+Qed.
+
+Lemma transEqTermNeu {Γ A t u v} {RA : [Γ ||-ne A]} :
+  [Γ ||-ne t ≅ u : A | RA] ->
+  [Γ ||-ne u ≅ v : A | RA] ->
+  [Γ ||-ne t ≅ v : A| RA].
+Proof.
+  intros [tL] [? tR]; exists tL tR; tea.
+  etransitivity; tea.
+  unshelve erewrite (redtmwf_det _ _ _ _ _ _ _ _ redR redL0); tea.
+  all: now apply whnf_whne.
+Qed.
+
+
+Lemma transEqTermΠ {Γ lA A t u v} {ΠA : [Γ ||-Π<lA> A]}
+  (ihdom : forall (Δ : context) (ρ : Δ ≤ Γ) (h : [ |-[ ta ] Δ]) (t u v : term),
+  [PiRedTyPack.domRed ΠA ρ h | Δ ||- t ≅ u : (PiRedTyPack.dom ΠA)⟨ρ⟩] ->
+  [PiRedTyPack.domRed ΠA ρ h | Δ ||- u ≅ v : (PiRedTyPack.dom ΠA)⟨ρ⟩] ->
+  [PiRedTyPack.domRed ΠA ρ h | Δ ||- t ≅ v : (PiRedTyPack.dom ΠA)⟨ρ⟩])
+  (ihcod : forall (Δ : context) (a : term) (ρ : Δ ≤ Γ) (h : [ |-[ ta ] Δ])
+   (ha : [PiRedTyPack.domRed ΠA ρ h | Δ ||- a : (PiRedTyPack.dom ΠA)⟨ρ⟩])
+   (t u v : term),
+  [PiRedTyPack.codRed ΠA ρ h ha | Δ ||- t ≅ u : (PiRedTyPack.cod ΠA) [a .: ρ >> tRel]] ->
+  [PiRedTyPack.codRed ΠA ρ h ha | Δ ||- u ≅ v : (PiRedTyPack.cod ΠA) [a .: ρ >> tRel]] ->
+  [PiRedTyPack.codRed ΠA ρ h ha | Δ ||- t ≅ v : (PiRedTyPack.cod ΠA) [a .: ρ >> tRel]]) :
+  [Γ ||-Π t ≅ u : A | PiRedTyPack.toPiRedTy ΠA ] ->
+  [Γ ||-Π u ≅ v : A | PiRedTyPack.toPiRedTy ΠA ] ->
+  [Γ ||-Π t ≅ v : A | PiRedTyPack.toPiRedTy ΠA ].
+Proof.
+  intros [tL] [? tR];
+  unshelve epose proof (e := redtmwf_det _ _ _ _ _ _ _ _ (PiRedTm.red redR) (PiRedTm.red redL)); tea.
+  1,2: apply isFun_whnf; apply PiRedTm.isfun.
+  exists tL tR.
+  + etransitivity; tea. now rewrite e.
+  + intros. eapply ihcod.
+    1: eapply eqApp.
+    rewrite e; apply eqApp0.
+Qed.
+
+Lemma transEqTerm@{h i j k l} {Γ lA A t u v} 
+  {RA : [LogRel@{i j k l} lA | Γ ||- A]} :
+  [Γ ||-<lA> t ≅ u : A | RA] ->
+  [Γ ||-<lA> u ≅ v : A | RA] ->
+  [Γ ||-<lA> t ≅ v : A | RA].
+Proof. 
+  revert t u v; pattern lA, Γ, A, RA; apply LR_rect_TyUr; clear lA Γ A RA; intros l Γ.
+  - intros *; apply transEqTermU@{h i j k}.
+  - intros *; apply transEqTermNeu.
+  - intros * ?????. apply transEqTermΠ; tea.
+Qed.
+
+End Transitivity.
