theories/LogicalRelation/Universe.v
@@ -1,0 +1,31 @@
+From LogRel.AutoSubst Require Import core unscoped Ast Extra.
+From LogRel Require Import Utils BasicAst Context Untyped Weakening GenericTyping LogicalRelation Reduction.
+From LogRel.LogicalRelation Require Import Irrelevance Induction.
+
+Set Universe Polymorphism.
+
+Section Universe.
+  Context `{GenericTypingProperties}.
+
+  Lemma univTmTy' {Γ l A} (h : [Γ ||-U l]) :
+    [Γ ||-<l> A : U | LRU_ h] -> [Γ ||-<URedTy.level h> A].
+  Proof.  intros []; now eapply RedTyRecFwd. Qed.
+
+  Lemma univTmTy {Γ l A} (RU : [Γ ||-<l> U]) :
+    [Γ ||-<l> A : U | RU] -> [Γ ||-<URedTy.level (invLRU RU)> A].
+  Proof. 
+    intros h; apply univTmTy'.
+    irrelevance.
+  Qed.
+
+  Lemma univEqTmEqTy' {Γ l l' A B} (h : [Γ ||-U l]) (RA : [Γ ||-<l'> A]) :
+    [Γ ||-<l> A ≅ B : U | LRU_ h] -> [Γ ||-<l'> A ≅ B | RA].
+  Proof. intros [????? RA']. apply TyEqRecFwd in RA'. irrelevance. Qed.
+
+  Lemma univEqTmEqTy {Γ l l' A B} (RU : [Γ ||-<l> U]) (RA : [Γ ||-<l'> A]) :
+    [Γ ||-<l> A ≅ B : U | RU] -> [Γ ||-<l'> A ≅ B | RA].
+  Proof. intros h; eapply (univEqTmEqTy' (invLRU RU)); irrelevance. Qed.
+
+End Universe.
+
+    
